more

Weidenbach_Book/Watched_Literals_List_Restart.thy
@@ -3,12 +3,9 @@ theory Watched_Literals_List_Restart
 begin
 
 text \<open>
-  Unlike most other refinements steps we have done, we don't try to produce here to refine our
-  specification to our code:
-  \<^item> It is not clear how to get closer to code we would like to have
-  \<^item> Without reasonable idea on the code, there are too many paths to produce a useful refinement
-    step (for example, if the we want to restart without changing the level, we probably don't
-    want to restart. This is can be expressed more easily later).
+  Unlike most other refinements steps we have done, we don't try to refine our
+  specification to our code directly: We first introduce an intermediate transition system which
+  is closer to what we want to implement. Then we refine it to code.
 \<close>
 
 text \<open>
@@ -1563,7 +1560,7 @@ definition remove_all_annot_true_clause_imp
   :: \<open>nat literal \<Rightarrow> nat twl_st_l \<Rightarrow> (nat twl_st_l) nres\<close>
 where
 \<open>remove_all_annot_true_clause_imp = (\<lambda>L (M, N, D, NE, UE, Q, W). do {
-    xs \<leftarrow> SPEC(\<lambda>xs. \<forall>x\<in>set xs. L \<in> set (N\<propto>x));
+    xs \<leftarrow> SPEC(\<lambda>xs. (\<forall>x\<in>set xs. x \<in># dom_m N \<longrightarrow> L \<in> set (N\<propto>x)));
     (_, N, NE) \<leftarrow> WHILE\<^sub>T
       (\<lambda>(i, N, NE). i < length xs)
       (\<lambda>(i, N, NE). do {
@@ -1761,7 +1758,7 @@ proof -
                                     (i + 1, M, N, D, NE, UE, WS, Q)) \<and>
                                 (s', s) \<in> measure (\<lambda>(i, N, NE). length xs - i)))\<close>
     if
-      xs: \<open>xs \<in> {xs. \<forall>x\<in>set xs. L \<in> set (N \<propto> x)}\<close> and
+      xs: \<open>xs \<in> {xs. (\<forall>x\<in>set xs. x \<in># dom_m N \<longrightarrow> L \<in> set (N \<propto> x))}\<close> and
       I: \<open>case s of (_, N, NE) \<Rightarrow>
          remove_one_annot_true_clause_inv U (i + 1, M, N, D, NE, UE, WS, Q)\<close> and
       cond: \<open>case s of (i, N, NE) \<Rightarrow> i < length xs\<close> and
@@ -1797,7 +1794,7 @@ proof -
       using lev0 rtranclp_remove_one_annot_true_clause_map_is_decided_trail[OF SU']
         rtranclp_remove_one_annot_true_clause_map_lit_of_trail[OF SU']
         trail_renumber_get_level[of \<open>get_trail_l S\<close> M L] by force
-    have \<open>reduce_dom_clauses (get_clauses_l (M, N, D, NE, UE, WS, Q))
+    have red: \<open>reduce_dom_clauses (get_clauses_l (M, N, D, NE, UE, WS, Q))
       (get_clauses_l (M, N', D, NE', UE, WS, Q))\<close>
       using rtranclp_remove_one_annot_true_clause_reduce_dom_clauses[OF UU'] unfolding U
       by simp
@@ -1820,7 +1817,9 @@ proof -
       apply (rule ccontr)
       using dom list_invs_U' by (auto simp: twl_list_invs_def)
     have L_set: \<open>L \<in> set (N \<propto> (xs!k))\<close>
-      using xs cond nth_mem[of k xs] unfolding s by (auto simp del: nth_mem)
+      using xs cond nth_mem[of k xs] dom red unfolding s reduce_dom_clauses_def
+      apply (auto simp del: nth_mem simp: )
+      sorry
     have \<open>no_dup M\<close>
       using n_d unfolding U by simp
     then have no_already_annot: \<open>Propagated Laa (xs ! k) \<in>  set M \<Longrightarrow> False\<close> for Laa
@@ -2410,7 +2409,7 @@ definition restart_prog_l :: "nat twl_st_l \<Rightarrow> nat \<Rightarrow> bool 
    }\<close>
 
 lemma restart_prog_l_restart_abs_l:
-  \<open>restart_prog_l S n brk \<le> \<Down> Id (restart_abs_l S n brk)\<close>
+  \<open>(uncurry2 restart_prog_l, uncurry2 restart_abs_l) \<in> Id \<times>\<^sub>f nat_rel \<times>\<^sub>f bool_rel \<rightarrow>\<^sub>f \<langle>Id\<rangle>nres_rel\<close>
 proof -
   have cdcl_twl_restart_l_prog: \<open>cdcl_twl_restart_l_prog S \<le> SPEC (cdcl_twl_restart_l S)\<close>
     if
@@ -2419,7 +2418,7 @@ proof -
       \<open>b \<in> {b. b \<longrightarrow> f n < size (get_learned_clss_l S)}\<close> and
       \<open>ba \<in> {b. b \<longrightarrow> f n < size (get_learned_clss_l S)}\<close> and
       brk: \<open>b \<and> \<not> brk\<close>
-    for b ba
+    for b ba S brk n
   proof -
     obtain T where
       ST: \<open>(S, T) \<in> twl_st_l None\<close> and
@@ -2439,14 +2438,91 @@ proof -
       by (rule conc_trans_additional)
   qed
 
-  show ?thesis
+  have \<open>restart_prog_l S n brk \<le> \<Down> Id (restart_abs_l S n brk)\<close> for S n brk
     unfolding restart_prog_l_def restart_abs_l_def restart_required_l_def
     apply (refine_vcg)
     subgoal by auto
     subgoal by (rule cdcl_twl_restart_l_prog)
     subgoal by auto
     done
+  then show ?thesis
+    apply -
+    unfolding uncurry_def
+    apply (intro frefI nres_relI)
+    by force
 qed
+
+definition cdcl_twl_stgy_restart_prog_l :: "nat twl_st_l \<Rightarrow> nat twl_st_l nres" where
+  \<open>cdcl_twl_stgy_restart_prog_l S\<^sub>0 =
+  do {
+    (brk, T, _) \<leftarrow> WHILE\<^sub>T\<^bsup>\<lambda>(brk, T, n). cdcl_twl_stgy_restart_abs_l_inv S\<^sub>0 brk T n\<^esup>
+      (\<lambda>(brk, _). \<not>brk)
+      (\<lambda>(brk, S, n).
+      do {
+        T \<leftarrow> unit_propagation_outer_loop_l S;
+        (brk, T) \<leftarrow> cdcl_twl_o_prog_l T;
+        (T, n) \<leftarrow> restart_prog_l T n brk;
+        RETURN (brk, T, n)
+      })
+      (False, S\<^sub>0, 0);
+    RETURN T
+  }\<close>
+
+lemma cdcl_twl_stgy_restart_prog_l_cdcl_twl_stgy_restart_abs_l:
+  \<open>(cdcl_twl_stgy_restart_prog_l, cdcl_twl_stgy_restart_abs_l) \<in> {(S, S').
+   (S, S') \<in> Id \<and>  twl_list_invs S \<and>  clauses_to_update_l S =  {#}} \<rightarrow>\<^sub>f \<langle>Id\<rangle> nres_rel\<close>
+   (is \<open>_ \<in> ?R \<rightarrow>\<^sub>f _\<close>)
+proof -
+  have [refine0]: \<open>((False, S, 0), (False, T , 0)) \<in> bool_rel \<times>\<^sub>r ?R \<times>\<^sub>r nat_rel\<close>
+    if \<open>(S, T) \<in> ?R\<close>
+    for S T
+    using that by auto
+  have [refine0]: \<open>unit_propagation_outer_loop_l x1c  \<le> \<Down> Id (unit_propagation_outer_loop_l x1a)\<close>
+    if \<open>(x1c, x1a) \<in> Id\<close>
+    for x1c x1a
+    using that by auto
+  have [refine0]: \<open>cdcl_twl_o_prog_l x1c  \<le> \<Down> Id (cdcl_twl_o_prog_l x1a)\<close>
+    if \<open>(x1c, x1a) \<in> Id\<close>
+    for x1c x1a
+    using that by auto
+  show ?thesis
+    unfolding cdcl_twl_stgy_restart_prog_l_def cdcl_twl_stgy_restart_prog_def uncurry_def
+      cdcl_twl_stgy_restart_abs_l_def
+    apply (intro frefI nres_relI)
+    apply (refine_rcg WHILEIT_refine[where R = \<open>{((brk :: bool, S, n :: nat), (brk', S', n')).
+        (S, S') \<in> Id \<and> brk = brk' \<and> n = n'}\<close>]
+        unit_propagation_outer_loop_l_spec[THEN fref_to_Down]
+        cdcl_twl_o_prog_l_spec[THEN fref_to_Down]
+        restart_abs_l_restart_prog[THEN fref_to_Down_curry2]
+        restart_prog_l_restart_abs_l[THEN fref_to_Down_curry2])
+    subgoal by auto
+    subgoal for x y xa x' x1 x2 x1a x2a
+      by fastforce
+    subgoal by auto
+    subgoal
+      by (simp add: twl_st_l twl_st)
+    subgoal by (auto simp: twl_st_l twl_st)
+    subgoal
+       unfolding cdcl_twl_stgy_restart_prog_inv_def cdcl_twl_stgy_restart_abs_l_inv_def
+       by (auto simp: twl_st_l twl_st)
+    subgoal by auto
+    done
+qed
+
+lemma cdcl_twl_stgy_restart_prog_l_cdcl_twl_stgy_restart_prog:
+ \<open>(cdcl_twl_stgy_restart_prog_l, cdcl_twl_stgy_restart_prog)
+  \<in> {(S, S'). (S, S') \<in> twl_st_l None \<and> twl_list_invs S \<and> clauses_to_update_l S = {#}} \<rightarrow>\<^sub>f
+   \<langle>{(S, S'). (S, S') \<in> twl_st_l None \<and> twl_list_invs S}\<rangle>nres_rel\<close>
+  apply (intro frefI nres_relI)
+  apply (rule order_trans)
+  defer
+  apply (rule cdcl_twl_stgy_restart_abs_l_cdcl_twl_stgy_restart_abs_l[THEN fref_to_Down])
+    apply fast
+    apply assumption
+  apply (rule cdcl_twl_stgy_restart_prog_l_cdcl_twl_stgy_restart_abs_l[THEN fref_to_Down,
+    simplified])
+  apply simp
+  done
 
 end
 
